Presburger.v
@@ -23,7 +23,7 @@ Definition indicator (b: bool) :=
 Fixpoint eval_aff (a: Aff) (m: total_map Z) :=
   match a with
   | AConst c => c
-  | AVar v => m v
+  | AVar v => eval_map m v
   | APlus a1 a2 => (eval_aff a1 m) + (eval_aff a2 m)
   | AMinus a1 a2 => (eval_aff a1 m) - (eval_aff a2 m)
   | AMul c a => c * (eval_aff a m)
@@ -32,6 +32,8 @@ Fixpoint eval_aff (a: Aff) (m: total_map Z) :=
 Class PresburgerImpl (PSet PwAff: Type) :=
   {
     eval_set : PSet -> total_map Z -> bool;
+    eval_set_same : forall m1 m2, (forall x, eval_map m1 x = eval_map m2 x) ->
+                             forall s, eval_set s m1 = eval_set s m2;
 
     empty_set : PSet;
     empty_set_spec : forall x, eval_set empty_set x = false;
@@ -143,18 +145,17 @@ Ltac simpl_eval_presburger :=
     ).
 
 Theorem constraint_eq_one_variable_correct {PSet PwAff: Type} {P: PresburgerImpl PSet PwAff} :
-  forall m p x, eval_set p m = eval_set (intersect_set (eq_set (pw_aff_from_aff (AVar x)) (pw_aff_from_aff (AConst (m x)))) p) m.
+  forall m p x, eval_set p m = eval_set (intersect_set (eq_set (pw_aff_from_aff (AVar x)) (pw_aff_from_aff (AConst (eval_map m x)))) p) m.
 Proof.
   move => m p x.
   by simpl_eval_presburger.
 Qed.
 
 Theorem constraint_neq_one_variable_correct {PSet PwAff: Type} {P: PresburgerImpl PSet PwAff} :
-  forall m x v, m x <> v ->
+  forall m x v, eval_map m x <> v ->
            forall p, eval_set p m = eval_set (intersect_set (ne_set (pw_aff_from_aff (AVar x)) (pw_aff_from_aff (AConst v))) p) m.
 Proof.
   move => m x v /Z.eqb_neq Hne p.
   simpl_eval_presburger.
   by rewrite Hne.
 Qed.
-
